aneris/examples/snapshot_isolation/proof/client_proxy/proof_of_init_client_proxy.v
@@ -1,0 +1,90 @@
+From iris.algebra Require Import auth gmap dfrac frac_auth excl csum.
+From iris.algebra.lib Require Import mono_list.
+From iris.base_logic Require Import invariants.
+From iris.bi.lib Require Import fractional.
+From iris.proofmode Require Import tactics coq_tactics reduction spec_patterns.
+From aneris.lib Require Import gen_heap_light.
+From aneris.aneris_lang Require Import lang resources inject tactics proofmode.
+From aneris.aneris_lang.lib Require Import list_proof lock_proof map_proof.
+From aneris.aneris_lang.lib.serialization Require Import serialization_proof.
+From aneris.aneris_lang.program_logic Require Import aneris_lifting.
+From aneris.aneris_lang.program_logic Require Import aneris_weakestpre.
+From aneris.examples.reliable_communication.lib.mt_server
+     Require Import user_params mt_server_code.
+From aneris.examples.reliable_communication.lib.mt_server.spec
+     Require Import api_spec.
+From aneris.examples.snapshot_isolation
+     Require Import snapshot_isolation_code.
+From aneris.examples.snapshot_isolation.specs
+     Require Import user_params resources specs.
+From aneris.examples.snapshot_isolation.proof
+     Require Import time events model kvs_serialization rpc_user_params.
+From aneris.examples.snapshot_isolation.proof.resources
+     Require Import
+     resource_algebras server_resources proxy_resources global_invariant wrappers.
+From aneris.examples.snapshot_isolation.instantiation
+     Require Import snapshot_isolation_api_implementation.
+Section Client_Proxy_Proof.
+
+  Context `{!anerisG Mdl Σ, !User_params, !IDBG Σ}.
+  Context (clients : gset socket_address).
+  Context (γKnownClients γGauth γGsnap γT : gname).
+  Context (srv_si : message → iProp Σ).
+  Notation MTC := (client_handler_rpc_user_params clients γKnownClients γGauth γGsnap γT).
+  Import snapshot_isolation_code_api.
+
+  Definition init_client_proxy_spec_internal {MTR : MTS_resources} : iProp Σ :=
+    ∀ (sa : socket_address),
+    {{{ unallocated {[sa]} ∗
+        KVS_address ⤇ srv_si ∗
+        sa ⤳ (∅, ∅) ∗
+        (@api_spec.init_client_proxy_spec _ _ _ _ MTC _ srv_si) ∗
+        client_can_connect_res γKnownClients sa ∗
+        free_ports (ip_of_address sa) {[port_of_address sa]} }}}
+      SI_init_client_proxy (s_serializer KVS_serialization)
+                  #sa #KVS_address @[ip_of_address sa]
+    {{{ cstate, RET cstate;
+        ConnectionState_def γKnownClients γGsnap γT cstate CanStart ∗
+        is_connected γGsnap γT γKnownClients cstate }}}.
+
+  Lemma init_client_leader_proxy_internal_holds {MTR : MTS_resources}  :
+     ⊢ init_client_proxy_spec_internal.
+  Proof.
+    iIntros (sa Φ) "!#".
+    iIntros "(Hf & #Hsi & Hmh & #Hspec & Hcc & Hfp) HΦ".
+    rewrite /SI_init_client_proxy /=.
+    rewrite /init_client_proxy.
+    wp_pures.
+    wp_apply ("Hspec" with "[$Hf $Hfp $Hmh $Hsi][Hcc HΦ]").
+    iNext.
+    iIntros (reqh) "Hreq".
+    wp_pures.
+    wp_alloc l as "Hl".
+    wp_pures.
+    iMod (own_alloc (Excl ())) as (γS) "Hs"; first done.
+    iMod (own_alloc (Excl ())) as (γA) "Ha"; first done.
+    iMod ghost_map.ghost_map_alloc_empty as (γCache) "HCache".
+    iDestruct "Hcc" as (γCst) "(#Hcc & Hp)".
+    wp_apply (newlock_spec
+                (KVS_InvName.@socket_address_to_str sa) _
+                (is_connected_def γGsnap γT (ip_of_address sa) reqh l PSCanStart (InjLV #()) γS γA γCache)
+               with "[Hreq Hl HCache Hs]").
+    - iFrame. iLeft. by iFrame.
+    - iIntros (lk γ) "#Hlk".
+      iMod (own_update _ _ (Cinr (to_agree (γA, γS, γ, γCache))) with "Hp") as "#Hdefined".
+      {  intros n [f |]; simpl; eauto.
+         destruct f; simpl; try by inversion 1. }
+      wp_pures.
+      iApply "HΦ".
+      iAssert (is_connected γGsnap γT γKnownClients (#sa, (lk, (reqh, #l)))) as "#Hic".
+      iExists _, _, _, _, _, _, _, _.
+      iExists _, _, _.
+      by iFrame "#∗".
+      rewrite /ConnectionState_def /connection_state.
+      iFrame "#∗".
+      iExists PSCanStart; iSplit; last done.
+      iExists sa, (lk, (reqh, #l))%V, γCst, γA, γS, γ, γCache.
+      by iFrame "#∗".
+  Qed.
+
+End Client_Proxy_Proof.
